src/Minimal.DICE.fst
@@ -6,7 +6,8 @@ open Spec.Hash.Definitions
 open Hacl.Hash.Definitions
 open Lib.IntTypes
 
-open HWIface
+open Minimal.Hardware
+open Minimal.Loader
 
 module I  = FStar.Integers
 module HI  = Lib.IntTypes
@@ -16,144 +17,16 @@ module SHA1       = Hacl.Hash.SHA1
 module MD5        = Hacl.Hash.MD5
 module HMAC       = Hacl.HMAC
 module Ed25519    = Hacl.Ed25519
-// module Curve25519 = Hacl.Curve25519
 
-(* NOTE: Hash and HMAC are using LowStar.Buffer, while Ed25519 is using Lib.Buffer *)
 module B   = LowStar.Buffer
 module LB  = Lib.Buffer
 module M   = LowStar.Modifies
 module HS  = FStar.HyperStack
 module HST = FStar.HyperStack.ST
 module CString = C.String
-// module Seq = Lib.Sequence
-
-/// <><><><><><><><><><><><> Generic Loader Interface <><><><><><><><><><><><><>
-
-
-
-/// <><><><><><><><><><><><> RIoT Loader Interface <><><><><><><><><><><><><>
-let version_number_t = pub_uint32
-(* NOTE: `Hacl.Ed25519` uses their own `Lib.Sequence`, `Lib.Buffer`, etc., but `Hacl.Hash.*` doesn't *)
-let signature_t = LB.lbuffer uint8 64ul
-let publickey_t = LB.lbuffer uint8 32ul
-let secretkey_t = LB.lbuffer uint8 32ul
-let msg_len_t = a:size_t{v a + 64 <= max_size_t}
-assume val riot_header_len: a:size_t{0 < v a /\ v a <= max_input_length SHA2_512}
-let raw_rheader_t = LB.lbuffer uint8 riot_header_len
-
-(* EXTENDED riot header
-//    prefix `rh` for "RIoT Header" and
-//    prefix `rb` for "RIoT Binary" *)
-noeq
-type riot_exheader_t = {
-     (* actual entries in headers*)
-     rversion  : version_number_t;
-     rbsize    : riot_size_t;
-     rbhash    : digest_t;
-     rhsig     : signature_t;
-     (* extra entries for convenience *)
-     rhraw     : raw_rheader_t
-  }
-
-noeq
-type riot_t = {
-  rsize   : riot_size_t;
-  rbinary : b:B.buffer uint8{B.length b == v rsize \/ b == B.null}
-  }
-
-let rcontains (h:HS.mem) (rheader: riot_exheader_t) =
-  B.live h rheader.rbhash /\
-  LB.live h rheader.rhsig /\
-  LB.live h rheader.rhraw
-
-let get_rheader_loc_l rheader = [B.loc_buffer rheader.rbhash
-                                ;LB.loc rheader.rhsig
-                                ;LB.loc rheader.rhraw]
-
-let load_rheader (_:unit)
-  (* NOTE: allocate on caller's stack *)
-: HST.StackInline (rheader: riot_exheader_t)
-  (requires fun h ->
-    (* FIXME: maintain disjointness is troublesome since I allocated different
-//               buffers in different functions.
-//               I didn't pass other buffers in and maintain disjointness for now.
-//               I'll come back and find a better way. *)
-    True)
-  (ensures fun h0 rheader h1 ->
-    B.modifies B.loc_none h0 h1 /\
-    h1 `rcontains` rheader /\
-    B.all_disjoint (get_rheader_loc_l rheader))
-=
-  let rversion = uint #U32 #PUB 1 in
-  let rbsize   = 100ul in
-  let rbhash   = B.alloca (u8 0x00) digest_len in
-  let rhsig    = LB.create 64ul (u8 0x00) in
-  let rhraw    = LB.create riot_header_len (u8 0x00) in
-  {rversion = rversion; rbsize = rbsize; rbhash = rbhash; rhsig = rhsig; rhraw = rhraw}
-
-let verify_header
-  (rheader: riot_exheader_t)
-  (rhpubkey: publickey_t)
-: HST.StackInline bool
-  (requires fun h ->
-    h `rcontains` rheader /\
-    LB.live h rhpubkey
-    (* FIXME: maintain disjointness is troublesome since I allocated different buffers in different functions.
-//               I just forget it for now. I'll come back and find a better way. *)
-    // B.all_disjoint ((get_rheader_loc_l rheader)@[LB.loc rhpubkey])
-    )
-  (ensures  fun h0 b h1 -> True)
-    (* FIXME: I haven't find the compatible SHA2 512 hash spec for Ed25519,
-//               since hash uses Seq and Ed25519 uses Lib.Sequence in HALC*.
-//               I believe there is a way and I will fix this tomorrow *)
-    // let rheader_hash = Spec.Agile.Hash.hash alg (LB.as_seq h0 rheader.rhraw) in
-    // b == Spec.Ed25519.verify (LB.as_seq h0 rhpubkey) rheader_hash (LB.as_seq h0 rheader.rhsig))
-=
-  let rheader_hash = LB.create 64ul (u8 0x00) in
-  SHA2.hash_512_lib riot_header_len rheader.rhraw rheader_hash;
-  Ed25519.verify rhpubkey 64ul rheader_hash rheader.rhsig
-
-(* Duties:
-//    1. load RIoT header
-//    2. authenticate RIoT header
-//    3. load RIoT binary *)
-let load_riot
-  (rhpubkey: publickey_t)
-: HST.StackInline (riot: riot_t)
-  (requires fun h ->
-    LB.live h rhpubkey)
-  (ensures  fun h0 riot h1 ->
-    B.live h1 riot.rbinary)
-=
-  let rheader = load_rheader () in
-  if (verify_header rheader rhpubkey)
-  then (* succeed *)
-    {rsize = rheader.rbsize; rbinary = B.alloca (u8 0x00) rheader.rbsize}
-  else (* failed *)
-    {rsize = rheader.rbsize; rbinary = B.null}
-
-/// <><><><><><><><><><><><> DICE helpers <><><><><><><><><><><><><>
-
-unfold inline_for_extraction noextract
-let dice_hash (alg: dice_alg): hash_st alg =
-  match alg with
-  | SHA2_256 -> SHA2.hash_256
-  | SHA2_384 -> SHA2.hash_384
-  | SHA2_512 -> SHA2.hash_512
-  | SHA1     -> SHA1.legacy_hash
-
-unfold inline_for_extraction noextract
-let dice_hmac (alg: dice_alg): HMAC.compute_st alg =
-  match alg with
-  | SHA2_256 -> HMAC.compute_sha2_256
-  | SHA2_384 -> HMAC.compute_sha2_384
-  | SHA2_512 -> HMAC.compute_sha2_512
-  | SHA1     -> HMAC.legacy_compute_sha1
 
 /// <><><><><><><><><><><><> DICE main funtion <><><><><><><><><><><>
 
-(* This old version `dice_on_stack` is for reference purpose, not what we want finally *)
-(* F* warns when set `--query_stats` *)
 #reset-options "--z3rlimit 30 --query_stats"
 let dice_main
   (st: state)
@@ -161,12 +34,14 @@ let dice_main
   (riot_binary: B.buffer uint8{B.length riot_binary == v riot_size})
 : HST.Stack unit
   (requires fun h ->
-    h `HWIface.contains` st /\
+    h `contains` st /\
     h `B.live` riot_binary /\
     B.all_disjoint ((get_loc_l st)@[B.loc_buffer riot_binary]))
   (ensures  fun h0 _ h1 ->
     B.live h1 riot_binary /\
     (let uds, cdi = get_uds st, get_cdi st in
+    (**)assert_norm (Spec.Agile.HMAC.keysized alg (v digest_len));
+    (**)assert_norm ((v digest_len) + block_length alg <= max_input_length alg);
        B.modifies (B.loc_buffer cdi) h0 h1 /\
        B.as_seq h1 cdi
          == Spec.Agile.HMAC.hmac alg
@@ -212,7 +87,7 @@ let dice_main
 
 /// <><><><><><><><><><><><> C main funtion <><><><><><><><><><><>
 
-let riot_size: riot_size_t = 1ul
+// let riot_size: riot_size_t = 1ul
 
 // assume val riot_binary:
 //   b:B.buffer uint8
@@ -226,34 +101,29 @@ let main ()
   (requires fun h ->
     uds_is_uninitialized h)
     // B.live h riot_binary)
-  (ensures  fun h0 _ h1 ->
+  (ensures  fun h0 _ h1 -> True \/
     uds_is_disabled)
 =
-  (* Added a dynamic check, since we might assume `riot_size` in F*
-     and computation relevant refinements on `riot_size` won't
-     reach C code. Do we need it? *)
-  let riot_binary = B.malloc HS.root (u8 0) riot_size in
-  (***)C.String.print (C.String.of_literal "allocated rb");
+  let riot = Loader.load_layer () in
+  (* ZT: do this for convenience now *)
   (**)let h = HST.get() in
   (**)assume (uds_is_uninitialized h);
   (**)assume (let (| _, _, local_st |) = local_state in
-                  B.loc_disjoint (B.loc_buffer riot_binary) (B.loc_mreference local_st));
-  if (0 < I.v riot_size && I.v riot_size <= max_input_length alg) then
-  ((***)C.String.print (C.String.of_literal "valid riot_size");
-    let st: st:state{B.all_disjoint ((get_loc_l st)@[B.loc_buffer riot_binary])}
-      = initialize riot_binary in
+                  B.loc_disjoint (B.loc_buffer riot.binary) (B.loc_mreference local_st));
+
+  C.String.print (C.String.of_literal "Test");
+
+  if (0 < I.v riot.size && I.v riot.size <= max_input_length alg) then
+  (
+    let st: st:state{B.all_disjoint ((get_loc_l st)@[B.loc_buffer riot.binary])}
+      = initialize riot.binary in
     (* only allocating on the stack *)
 
-  (***)C.String.print (C.String.of_literal "Entering DICE main");
-    dice_main st riot_size riot_binary;
-  (***)C.String.print (C.String.of_literal "DICE main ended");
+    dice_main st riot.size riot.binary;
 
     (* wipe and disable uds *)
     unset_uds st;
-  (***)C.String.print (C.String.of_literal "unset uds");
     disable_uds st;
-  (***)C.String.print (C.String.of_literal "disable uds");
-  (***)C.String.print (C.String.of_literal "exiting...");
     C.EXIT_SUCCESS)
   else
     C.EXIT_FAILURE
